More on repeat invariant

iodiv/DivFreeTauSpec.fst
@@ -474,6 +474,10 @@ unfold
 let iprepost #a (pre : history -> Type0) (post : (hist : history) -> orun a -> Pure Type0 (requires pre hist) (ensures fun _ -> True)) : iwp a =
   fun p hist -> pre hist /\ (forall r. post hist r ==> p r)
 
+let iprepost_inst #a (pre : history -> Type0) (post : (hist : history) -> orun a -> Pure Type0 (requires pre hist) (ensures fun _ -> True)) (p : i_post a) h r :
+  Lemma (requires iprepost pre post p h /\ post h r) (ensures p r)
+= ()
+
 (** Basic predicates *)
 
 unfold
@@ -519,6 +523,48 @@ let sotrace_refines (s : sotrace) (trs : stream trace) =
 unfold
 let repeat_inv #index (pre : index -> i_pre) (inv : trace -> Type0) (i : index) : iwp unit =
   iprepost (pre i) (fun hist r -> diverges r /\ (exists (trs : stream trace). (forall n. inv (trs n)) /\ (inf_trace r) `sotrace_refines` trs))
+
+let repeat_inv_inst #index (pre : index -> i_pre) (inv : trace -> Type0) (i : index) (post : i_post unit) hist (s : sotrace) (trs : stream trace) :
+  Lemma (requires repeat_inv pre inv i post hist /\ (forall n. inv (trs n)) /\ s `sotrace_refines` trs) (ensures post (Odv s))
+= ()
+
+let repeat_inv_expand_aux #index (pre : index -> i_pre) (inv : trace -> Type0) (post : i_post unit) (hist : history) (j : index) (tr : otrace) (trs : stream trace) (s : sotrace) :
+  Lemma
+    (requires repeat_inv pre inv j post hist /\ (forall n. inv (trs n)) /\ s `sotrace_refines` trs)
+    (ensures post (Odv (stream_prepend tr (stream_prepend [ None ] s))))
+= admit ()
+
+let repeat_inv_expand #index (pre : index -> i_pre) (inv : trace -> Type0) (post : i_post unit) (hist : history) (j : index) (tr : otrace) :
+  Lemma
+    (requires repeat_inv pre inv j post hist /\ pre j (rev_acc (to_trace tr) hist))
+    (ensures repeat_inv pre inv j (ishift_post [ None ] (ishift_post tr post)) (rev_acc (to_trace tr) hist))
+= introduce forall r. diverges r /\ (exists (trs : stream trace). (forall n. inv (trs n)) /\ (inf_trace r) `sotrace_refines` trs) ==> ishift_post [ None ] (ishift_post tr post) r
+  with begin
+    introduce diverges r /\ (exists (trs : stream trace). (forall n. inv (trs n)) /\ (inf_trace r) `sotrace_refines` trs) ==> ishift_post [ None ] (ishift_post tr post) r
+    with _. begin
+      match r with
+      | Odv s ->
+        eliminate exists (trs : stream trace). (forall n. inv (trs n)) /\ (inf_trace r) `sotrace_refines` trs
+        returns ishift_post [ None ] (ishift_post tr post) (Odv s)
+        with _. begin
+          // calc (==) {
+          //   ishift_post [ None ] (ishift_post tr post) (Odv s) ;
+          //   == {}
+          //   ishift_post tr post (Odv (stream_prepend [ None ] s)) ;
+          //   == {}
+          //   post (Odv (stream_prepend tr (stream_prepend [ None ] s))) ;
+          // } ;
+          // let trs' = stream_prepend [ to_trace tr ] trs in
+          // assume (forall n. inv (trs' n)) ;
+          // assume ((stream_prepend tr (stream_prepend [ None ] s)) `sotrace_refines` trs') ;
+          // repeat_inv_inst pre inv j post hist (stream_prepend tr (stream_prepend [ None ] s)) trs' ;
+          // assert (repeat_inv pre inv j post hist) ; // Seems I need to revoke the unfold status of repeat_inv
+          assert ((forall n. inv (trs n)) /\ s `sotrace_refines` trs) ;
+          assume (post (Odv (stream_prepend tr (stream_prepend [ None ] s))))
+          // repeat_inv_expand_aux pre inv post hist j tr trs s
+        end
+    end
+  end
 
 let repeat_inv_proof #index (pre : index -> i_pre) (inv : trace -> Type0) (i : index) :
   Lemma (i_iter (repeat_body_inv pre inv) i `ile` repeat_inv pre inv i)
